State.v

theories/Interp/State.v
@@ -23,12 +23,12 @@ Set Implicit Arguments.
 
 #[global] Instance MonadTrigger_stateT {E S M} {MM : Monad M} {MT: MonadTrigger E M} :
   MonadTrigger E (stateT S M) :=
-  fun _ e s => v <- mtrigger _ e;; ret (s, v).
+  fun _ e s => v <- mtrigger e;; ret (s, v).
 
-Definition interp_state {E C M} S
+Definition fold_state {E C M} S
            {FM : Functor M} {MM : Monad M} {IM : MonadIter M}
            (h : E ~> stateT S M) (h' : bool -> C ~> stateT S M) :
-  ctree E C ~> stateT S M := interp h h'.
+  ctree E C ~> stateT S M := fold h h'.
 
 Section State.
   Variable (S : Type).
@@ -54,7 +54,7 @@ Section State.
 
   Definition run_state {E C} `{B1 -< C}
     : ctree (stateE +' E) C ~> stateT S (ctree E C) :=
-    interp_state (case_ h_state pure_state) pure_state_choice.
+    fold_state (case_ h_state pure_state) pure_state_choice.
 
 End State.
 
@@ -71,7 +71,7 @@ Section State.
           (h' : bool -> C ~> stateT S (ctree F D)).
 
   (** Facts about state (equational theory) *)
-  Definition _interp_state
+  Definition _fold_state
              (h  : E ~> stateT S (ctree F D))
              (h' : bool -> C ~> stateT S (ctree F D))
              (ot : ctreeF E C R (ctree E C R)) :
@@ -79,20 +79,20 @@ Section State.
     fun s =>
       match ot with
       | RetF r        => Ret (s, r)
-      | BrF b c k => h' b _ c s >>= fun sx => Guard (interp_state h h' (k (snd sx)) (fst sx))
-      | VisF e k      => h _ e s    >>= fun sx => Guard (interp_state h h' (k (snd sx)) (fst sx))
+      | BrF b c k => h' b _ c s >>= fun sx => Guard (fold_state h h' (k (snd sx)) (fst sx))
+      | VisF e k      => h _ e s    >>= fun sx => Guard (fold_state h h' (k (snd sx)) (fst sx))
       end.
 
   Lemma interp_interp_state (t : ctree E C R) (s : S) :
-    interp h h' t s ≅ interp_state h h' t s.
+    fold h h' t s ≅ fold_state h h' t s.
   Proof.
     reflexivity.
   Qed.
 
-  Lemma unfold_interp_state t s :
-    interp_state h h' t s ≅ _interp_state h h' (observe t) s.
+  Lemma unfold_fold_state t s :
+    fold_state h h' t s ≅ _fold_state h h' (observe t) s.
   Proof.
-    unfold interp_state, interp, Basics.iter, MonadIter_stateT0, Basics.iter, MonadIter_ctree; cbn.
+    unfold fold_state, fold, Basics.iter, MonadIter_stateT0, Basics.iter, MonadIter_ctree; cbn.
     rewrite unfold_iter; destruct observe eqn:Hobs; cbn.
     - rewrite 2 bind_ret_l; reflexivity.
     - rewrite bind_map, bind_bind; cbn; setoid_rewrite bind_ret_l.
@@ -109,49 +109,48 @@ Section State.
   #[global]
   Instance equ_interp_state:
     Proper (equ eq ==> eq ==> equ eq)
-           (@interp_state _ _ _ _ _ _ _ h h' R).
+           (@fold_state _ _ _ _ _ _ _ h h' R).
   Proof.
     unfold Proper, respectful.
     coinduction ? IH; intros * EQ1 * <-.
-    rewrite !unfold_interp_state.
-    step in EQ1; inv EQ1; cbn [_interp_state]; auto.
+    rewrite !unfold_fold_state.
+    step in EQ1; inv EQ1; cbn [_fold_state]; auto.
     - simpl bind. upto_bind_eq.
       constructor; intros; auto.
     - simpl bind. upto_bind_eq.
       constructor; auto.
   Qed.
 
-  Lemma interp_state_ret
+  Lemma fold_state_ret
         (s : S) (r : R) :
-    (interp_state h h' (Ret r) s) ≅ (Ret (s, r)).
+    (fold_state h h' (Ret r) s) ≅ (Ret (s, r)).
   Proof.
     rewrite ctree_eta. reflexivity.
   Qed.
 
-  Lemma interp_state_vis {T : Type}
+  Lemma fold_state_vis {T : Type}
   (e : E T) (k : T -> ctree E C R) (s : S)
-    : interp_state h h' (Vis e k) s
-                   ≅ h e s >>= fun sx => Guard (interp_state h h' (k (snd sx)) (fst sx)).
+    : fold_state h h' (Vis e k) s
+                   ≅ h e s >>= fun sx => Guard (fold_state h h' (k (snd sx)) (fst sx)).
   Proof.
-    rewrite unfold_interp_state; reflexivity.
+    rewrite unfold_fold_state; reflexivity.
   Qed.
 
-  Lemma interp_state_br {T: Type} `{C -< D }
+  Lemma fold_state_br {T: Type} `{C -< D}
         (b : bool) (c : C T) (k : T -> ctree E C R) (s : S)
-    : interp_state h h' (br b c k) s
-                   ≅ br b c (fun sx => Guard (interp_state h h' (k sx) s)).
+    : fold_state h h' (br b c k) s
+                   ≅ h' b c s >>= fun sx => Guard (fold_state h h' (k (snd sx)) (fst sx)). 
   Proof.
-    rewrite !unfold_interp_state; simpl.
-    (* Lef: This looks wrong? *)
-  Abort.
+    rewrite !unfold_fold_state; reflexivity.
+  Qed.
 
-  Lemma interp_state_tau `{B1 -< C}
+  Lemma fold_state_tau `{B1 -< C}
         (t : ctree E C R) (s : S)
-        : interp_state h h' (Guard t) s ≅ Guard (Guard (interp_state h h' t s)).
+        : fold_state h h' (Guard t) s ≅ Guard (Guard (fold_state h h' t s)).
   Proof.
-    rewrite unfold_interp_state.
+    rewrite unfold_fold_state.
     simpl.
-    (* LEF: This was already aborted *)
+    (* LEF: This was already aborted, I don't think it's salvagable? *)
   Abort.
 
 End State.
@@ -168,25 +167,25 @@ Section State.
           (h : E ~> stateT S (ctree F D))
           (h' : bool -> C ~> stateT S (ctree F D)).
 
-  Lemma interp_state_trigger_eqit
+  Lemma fold_state_trigger_eqit
         (e : E R) (s : S)
-    : (interp_state h h' (CTree.trigger e) s) ≅ (h e s >>= fun x => Guard (Ret x)).
+    : (fold_state h h' (CTree.trigger e) s) ≅ (h e s >>= fun x => Guard (Ret x)).
   Proof.
-    unfold CTree.trigger. rewrite interp_state_vis; cbn.
+    unfold CTree.trigger. rewrite fold_state_vis; cbn.
     upto_bind_eq.
     (* TODO: why is this rewrite so slow?
        TODO: proof system for [equ] similar to the one for [sbisim]
      *)
     step. constructor. intros.
-    rewrite interp_state_ret.
+    rewrite fold_state_ret.
     now destruct x1.
   Qed.
 
-  Lemma interp_state_trigger `{B0 -< D}
+  Lemma fold_state_trigger `{B0 -< D}
         (e : E R) (s : S)
-    : interp_state h h' (CTree.trigger e) s ~ h e s.
+    : fold_state h h' (CTree.trigger e) s ~ h e s.
   Proof.
-    unfold CTree.trigger. rewrite interp_state_vis.
+    unfold CTree.trigger. rewrite fold_state_vis.
     rewrite <- (bind_ret_r (h e s)).
     match goal with
       |- ?y ~ ?x => remember y; rewrite <- (bind_ret_r x); subst
@@ -195,33 +194,33 @@ Section State.
     (* LEF: Why does it introduce two binders? *)
     upto_bind_eq.
     intros [ys yr].
-    rewrite sb_guard, interp_state_ret.
+    rewrite sb_guard, fold_state_ret.
     Fail now destruct x.
   Admitted.
 
-  Lemma interp_state_bind {A B}
+  Lemma fold_state_bind {A B}
         (t : ctree E C A) (k : A -> ctree E C B)
         (s : S) :
-    (interp_state h h' (t >>= k) s) 
+    (fold_state h h' (t >>= k) s) 
       ≅
-      (interp_state h h' t s >>= fun st => interp_state h h' (k (snd st)) (fst st)).
+      (fold_state h h' t s >>= fun st => fold_state h h' (k (snd st)) (fst st)).
   Proof.
     revert s t.
     coinduction ? IH; intros.
     rewrite (ctree_eta t).
     cbn.
     rewrite unfold_bind.
-    rewrite unfold_interp_state.
+    rewrite unfold_fold_state.
     destruct (observe t) eqn:Hobs; cbn.
-    - rewrite interp_state_ret. rewrite bind_ret_l. cbn.
-      rewrite unfold_interp_state. reflexivity.
-    - rewrite interp_state_vis.
+    - rewrite fold_state_ret. rewrite bind_ret_l. cbn.
+      rewrite unfold_fold_state. reflexivity.
+    - rewrite fold_state_vis.
       cbn.
       rewrite bind_bind. cbn.
       upto_bind_eq.
       rewrite bind_guard.
       constructor; intros ?; apply IH.
-    - rewrite unfold_interp_state.
+    - rewrite unfold_fold_state.
       cbn.
 
       rewrite bind_bind.
@@ -230,16 +229,16 @@ Section State.
       constructor; intros ?; apply IH.
   Qed.
 
-  (** LEF: This looks like it depends on [SBisimInterp.v] *)
+  (** LEF: This looks like it depends on [SBisimInterp.v]? Move there? *)
   (*
-Lemma trans0_interp_state : forall {E F X} (h : E ~> stateT S (ctree F)) (t t' : ctree E X) s,
-  trans0 t t' -> trans0 (interp_state h t s) (interp_state h t' s).
+Lemma trans0_fold_state : forall {E F X} (h : E ~> stateT S (ctree F)) (t t' : ctree E X) s,
+  trans0 t t' -> trans0 (fold_state h t s) (fold_state h t' s).
 Proof.
   intros. red in H. setoid_rewrite (ctree_eta t). setoid_rewrite (ctree_eta t').
   genobs t ot. genobs t' ot'. clear t Heqot t' Heqot'.
   induction H.
   - constructor. rewrite H. reflexivity.
-  - rewrite unfold_interp_state. cbn.
+  - rewrite unfold_fold_state. cbn.
     apply T0Br with (x := x).
     apply T0Br with (x := Fin.F1). apply IHtrans0_.
 Qed.
@@ -326,62 +325,62 @@ Qed.
 
 Lemma transis_trans {E F X} (h : E ~> stateT S (ctree F)) (Hh : forall X e s, vsimple (h X e s)) :
   forall l s s' (t t' : ctree E X),
-  transi_state h l s s' t t' -> exists t0, trans l (interp_state h t s) t0 /\ t0_det t0 (interp_state h t' s').
+  transi_state h l s s' t t' -> exists t0, trans l (fold_state h t s) t0 /\ t0_det t0 (fold_state h t' s').
 Proof.
   intros. induction H.
   - exists CTree.stuckD. apply trans_val_inv in H as ?.
     apply trans_val_trans0 in H as [].
-    eapply trans0_interp_state in H. rewrite interp_state_ret in H. setoid_rewrite H0.
-    setoid_rewrite interp_state_br. setoid_rewrite br0_always_stuck.
+    eapply trans0_fold_state in H. rewrite fold_state_ret in H. setoid_rewrite H0.
+    setoid_rewrite fold_state_br. setoid_rewrite br0_always_stuck.
     eapply trans0_trans in H; etrans. split; etrans. now left.
-  - exists (Guard (interp_state h t' s)). split; [| eright; eauto; now left ].
+  - exists (Guard (fold_state h t' s)). split; [| eright; eauto; now left ].
     apply trans_tau_trans0 in H as (? & ? & ? & ? & ?).
-    eapply trans0_interp_state in H. setoid_rewrite H0. eapply trans0_trans; etrans.
-    setoid_rewrite interp_state_br.
+    eapply trans0_fold_state in H. setoid_rewrite H0. eapply trans0_trans; etrans.
+    setoid_rewrite fold_state_br.
     econstructor. reflexivity.
-  - exists (x <- t'';; Guard (interp_state h t' s')).
+  - exists (x <- t'';; Guard (fold_state h t' s')).
     split. 2: { eapply t0_det_bind_ret_l; eauto. eright; eauto. now left. }
     apply trans_obs_trans0 in H as (? & ? & ?).
-    eapply trans0_interp_state in H. setoid_rewrite H2. eapply trans0_trans; etrans.
-    setoid_rewrite interp_state_vis.
-    eapply trans_bind_l with (k := fun sx => Guard (interp_state h (x0 (snd sx)) (fst sx))) in H1.
+    eapply trans0_fold_state in H. setoid_rewrite H2. eapply trans0_trans; etrans.
+    setoid_rewrite fold_state_vis.
+    eapply trans_bind_l with (k := fun sx => Guard (fold_state h (x0 (snd sx)) (fst sx))) in H1.
     setoid_rewrite t0_det_bind_ret_l_equ in H1 at 2; eauto. cbn in *. eapply H1.
     { intro. inv H3. apply trans_val_inv in H1. rewrite H1 in H0. inv H0. step in H3. inv H3. step in H4. inv H4. }
   - destruct IHtransi_state as (? & ? & ?).
     destruct (Hh Y e s). 2: { destruct H4. rewrite H4 in H1. apply trans_vis_inv in H1 as (? & ? & ?). step in H1. inv H1. }
     destruct H4. rewrite H4 in H1. inv_trans. subst.
     exists x0. split. 2: auto.
-    apply trans_obs_trans0 in H as (? & ? & ?). eapply trans0_interp_state in H.
-    setoid_rewrite interp_state_vis in H. setoid_rewrite H4 in H. setoid_rewrite bind_ret_l in H.
+    apply trans_obs_trans0 in H as (? & ? & ?). eapply trans0_fold_state in H.
+    setoid_rewrite fold_state_vis in H. setoid_rewrite H4 in H. setoid_rewrite bind_ret_l in H.
     eapply trans0_trans; etrans. setoid_rewrite <- H1. etrans.
 Qed.
 
-(** Various lemmas for the proof that interp_state preserves sbisim in some cases. *)
+(** Various lemmas for the proof that fold_state preserves sbisim in some cases. *)
 
-Lemma interp_state_ret_inv {E F X} (h : E ~> stateT S (ctree F)) : forall s (t : ctree E X) r,
-  interp_state h t s ≅ Ret r -> t ≅ Ret (snd r) /\ s = fst r.
+Lemma fold_state_ret_inv {E F X} (h : E ~> stateT S (ctree F)) : forall s (t : ctree E X) r,
+  fold_state h t s ≅ Ret r -> t ≅ Ret (snd r) /\ s = fst r.
 Proof.
   intros. setoid_rewrite (ctree_eta t) in H. setoid_rewrite (ctree_eta t).
   destruct (observe t) eqn:?.
-  - rewrite interp_state_ret in H. step in H. inv H. split; reflexivity.
-  - rewrite interp_state_vis in H. apply ret_equ_bind in H as (? & ? & ?). step in H0. inv H0.
-  - rewrite interp_state_br in H. step in H. inv H.
+  - rewrite fold_state_ret in H. step in H. inv H. split; reflexivity.
+  - rewrite fold_state_vis in H. apply ret_equ_bind in H as (? & ? & ?). step in H0. inv H0.
+  - rewrite fold_state_br in H. step in H. inv H.
 Qed.
 
-Lemma trans_interp_state_inv_gen {E F X Y} (h : E ~> stateT S (ctree F)) (Hh : forall X e s, vsimple (h X e s)) :
+Lemma trans_fold_state_inv_gen {E F X Y} (h : E ~> stateT S (ctree F)) (Hh : forall X e s, vsimple (h X e s)) :
   forall l s (k : Y -> ctree E X) t' (pre : ctree F Y),
   is_simple pre ->
-  trans l (x <- pre;; interp_state h (k x) s) t' ->
-  exists t0 s', t0_det t' (interp_state h t0 s') /\
+  trans l (x <- pre;; fold_state h (k x) s) t' ->
+  exists t0 s', t0_det t' (fold_state h t0 s') /\
   ((exists l t1 x, trans l pre t1 /\ t0_det t1 (Ret x : ctree F Y) /\ t0 ≅ k x) \/
-    exists (x : Y), trans (val x) pre CTree.stuckD /\ trans l (interp_state h (k x) s) t' /\ transi_state h l s s' (k x) t0).
+    exists (x : Y), trans (val x) pre CTree.stuckD /\ trans l (fold_state h (k x) s) t' /\ transi_state h l s s' (k x) t0).
 Proof.
   intros * Hpre H.
-  do 3 red in H. remember (observe (x <- pre;; interp_state h (k x) s)) as oi.
+  do 3 red in H. remember (observe (x <- pre;; fold_state h (k x) s)) as oi.
   setoid_rewrite (ctree_eta t') at 1.
   setoid_rewrite (ctree_eta t') at 2.
   genobs t' ot'. clear t' Heqot'.
-  assert (go oi ≅ x <- pre;; interp_state h (k x) s).
+  assert (go oi ≅ x <- pre;; fold_state h (k x) s).
   { rewrite Heqoi, <- ctree_eta. reflexivity. } clear Heqoi.
   revert Y s k pre Hpre H0. induction H; intros.
   - destruct n. now apply Fin.case0.
@@ -389,8 +388,8 @@ Proof.
     destruct H1 as [[] | (? & ? & ?)].
     + rewrite H1 in H0. setoid_rewrite bind_ret_l in H0. setoid_rewrite H1. clear pre Hpre H1.
       rewrite (ctree_eta (k0 x0)) in H0. destruct (observe (k0 x0)) eqn:?.
-      * rewrite interp_state_ret in H0. step in H0. inv H0.
-      * rewrite interp_state_vis in H0. apply br_equ_bind in H0 as ?. destruct H1 as [[] | (? & ? & ?)].
+      * rewrite fold_state_ret in H0. step in H0. inv H0.
+      * rewrite fold_state_vis in H0. apply br_equ_bind in H0 as ?. destruct H1 as [[] | (? & ? & ?)].
         --setoid_rewrite H1 in H0. setoid_rewrite bind_ret_l in H0.
           apply equ_br_invT in H0 as ?. destruct H2 as [? _]. apply eq_add_S in H2 as <-.
           simple apply equ_br_invE with (x := x) in H0.
@@ -404,13 +403,13 @@ Proof.
             inv H4. step in H3. inv H3. step in H6. inv H6. }
           destruct H3 as (_ & _ & ? & ?). exists x0. split. etrans. split.
           ++setoid_rewrite (ctree_eta (k0 x0)). rewrite Heqc.
-            setoid_rewrite interp_state_vis. setoid_rewrite H1. setoid_rewrite bind_ret_l. apply trans_guard. apply H3.
+            setoid_rewrite fold_state_vis. setoid_rewrite H1. setoid_rewrite bind_ret_l. apply trans_guard. apply H3.
           ++setoid_rewrite (ctree_eta (k0 x0)). rewrite Heqc. destruct x1.
              eapply transis_obs0. etrans. 2: { rewrite H1. etrans. } cbn in H4. cbn in *. etrans.
         --destruct (Hh X0 e s).
           destruct H3. rewrite H3 in H1. step in H1. inv H1.
           destruct H3. rewrite H3 in H1. step in H1. inv H1.
-      * rewrite interp_state_br in H0.
+      * rewrite fold_state_br in H0.
         apply equ_br_invT in H0 as ?. destruct H1 as [-> ->].
         simple apply equ_br_invE with (x := x) in H0 as ?.
         specialize (IHtrans_ _ s (fun _ : unit => k1 x) (Guard (Ret tt))).
@@ -422,7 +421,7 @@ Proof.
           inv H4. step in H3. inv H3. step in H5. inv H5. }
         destruct H3 as (? & ? & ? & ?).
         exists x1, x2. split; auto. right. exists x0. split; etrans. split.
-        rewrite (ctree_eta (k0 x0)), Heqc, interp_state_br.
+        rewrite (ctree_eta (k0 x0)), Heqc, fold_state_br.
         eapply trans_brD. 2: reflexivity. apply trans_guard. apply H4.
         rewrite (ctree_eta (k0 x0)), Heqc. eapply transis_brD; etrans.
     + specialize (IHtrans_ _ s k0 (x0 x)).
@@ -436,21 +435,21 @@ Proof.
     symmetry in H0. apply br_equ_bind in H0 as ?. destruct H1 as [[] | (? & ? & ?)].
     + rewrite H1 in H0. setoid_rewrite bind_ret_l in H0.
       rewrite (ctree_eta (k0 x0)) in H0. destruct (observe (k0 x0)) eqn:?.
-      * rewrite interp_state_ret in H0. step in H0. inv H0.
-      * rewrite interp_state_vis in H0. apply br_equ_bind in H0 as ?.
+      * rewrite fold_state_ret in H0. step in H0. inv H0.
+      * rewrite fold_state_vis in H0. apply br_equ_bind in H0 as ?.
         destruct H2 as [[] | (? & ? & ?)].
         { rewrite H2 in H0. setoid_rewrite bind_ret_l in H0. step in H0. inv H0. }
         pose proof (trans_brS x1 x). rewrite <- H2 in H4.
         edestruct Hh. { destruct H5. rewrite H5 in H4. inv_trans. }
         destruct H5. rewrite H5 in H4. apply trans_vis_inv in H4 as (? & ? & ?). discriminate.
-      * rewrite interp_state_br in H0.
+      * rewrite fold_state_br in H0.
         apply equ_br_invT in H0 as ?. destruct H2 as [-> ->].
         simple eapply equ_br_invE in H0 as ?. rewrite H in H2.
         exists (k1 x), s. symmetry in H2. split.
         { rewrite <- ctree_eta. rewrite H2. eapply t0_det_tau; auto. apply t0_det_id; auto. }
         right. exists x0. rewrite H1. split; etrans.
         split; setoid_rewrite (ctree_eta (k0 x0)); setoid_rewrite Heqc.
-        { setoid_rewrite interp_state_br. rewrite H2.
+        { setoid_rewrite fold_state_br. rewrite H2.
           econstructor. now rewrite <- ctree_eta. }
         econstructor; etrans.
     + pose proof (trans_brS x0 x).
@@ -464,8 +463,8 @@ Proof.
   - symmetry in H0. apply vis_equ_bind in H0 as ?. destruct H1 as [[] | (? & ? & ?)].
     + rewrite H1 in H0. setoid_rewrite bind_ret_l in H0.
      rewrite (ctree_eta (k0 x0)) in H0. destruct (observe (k0 x0)) eqn:?.
-      * rewrite interp_state_ret in H0. step in H0. inv H0.
-      * rewrite interp_state_vis in H0. apply vis_equ_bind in H0 as ?.
+      * rewrite fold_state_ret in H0. step in H0. inv H0.
+      * rewrite fold_state_vis in H0. apply vis_equ_bind in H0 as ?.
         destruct H2 as [[] | (? & ? & ?)].
         { rewrite H2 in H0. setoid_rewrite bind_ret_l in H0. step in H0. inv H0. }
         pose proof (trans_vis e x x1). rewrite <- H2 in H4.
@@ -480,10 +479,10 @@ Proof.
         right.
         exists x0. rewrite H1. split; etrans.
         split; setoid_rewrite (ctree_eta (k0 x0)); setoid_rewrite Heqc.
-        { setoid_rewrite interp_state_vis. rewrite H5. setoid_rewrite bind_vis.
+        { setoid_rewrite fold_state_vis. rewrite H5. setoid_rewrite bind_vis.
           econstructor. rewrite bind_ret_l. rewrite <- H3, <- ctree_eta. reflexivity. }
         eapply transis_obs; etrans. 2: { rewrite H5. etrans. } destruct x. now left.
-      * rewrite interp_state_br in H0. step in H0. inv H0.
+      * rewrite fold_state_br in H0. step in H0. inv H0.
     + pose proof (trans_vis e x x0).
       rewrite <- H1 in H3. edestruct Hpre.
       { apply H4 in H3. inv H3. }
@@ -493,46 +492,46 @@ Proof.
       { rewrite <- ctree_eta, H2. eapply t0_det_bind_ret_l; eauto. now left. }
       left. exists (obs e x), (x0 x), x1. split; auto. rewrite H1. etrans.
      - exists (CTree.stuckD), (fst r). split.
-       + left. unfold CTree.stuckD. rewrite interp_state_br.
+       + left. unfold CTree.stuckD. rewrite fold_state_br.
          rewrite !br0_always_stuck. reflexivity.
        + right. symmetry in H0. apply ret_equ_bind in H0 as (? & ? & ?).
          exists x. rewrite H. split; etrans. split.
          rewrite H0. rewrite br0_always_stuck. etrans.
-         apply interp_state_ret_inv in H0 as []. subst. rewrite H0. destruct r. cbn. apply transis_val. econstructor; etrans.
+         apply fold_state_ret_inv in H0 as []. subst. rewrite H0. destruct r. cbn. apply transis_val. econstructor; etrans.
 Qed.
 
-Lemma trans_interp_state_inv {E F X} (h : E ~> stateT S (ctree F)) (Hh : forall X e s, vsimple (h X e s)) :
+Lemma trans_fold_state_inv {E F X} (h : E ~> stateT S (ctree F)) (Hh : forall X e s, vsimple (h X e s)) :
   forall l (t : ctree E X) t' s,
-  trans l (interp_state h t s) t' ->
-  exists l t0 s', t0_det t' (interp_state h t0 s') /\ transi_state h l s s' t t0.
+  trans l (fold_state h t s) t' ->
+  exists l t0 s', t0_det t' (fold_state h t0 s') /\ transi_state h l s s' t t0.
 Proof.
   intros.
-   assert (trans l (Guard (Ret tt);; interp_state h t s) t').
+   assert (trans l (Guard (Ret tt);; fold_state h t s) t').
    { cbn. etrans. }
-  eapply trans_interp_state_inv_gen in H0; eauto. destruct H0 as (? & ? & ? & ?).
+  eapply trans_fold_state_inv_gen in H0; eauto. destruct H0 as (? & ? & ? & ?).
   destruct H1 as [(? & ? & ? & ? & ? & ?) | (? & ? & ? & ?)].
   - inv_trans. subst. inv H2. step in H1. inv H1. step in H3. inv H3.
   - inv_trans. subst. eauto.
   - left. intros. inv_trans. subst. constructor.
 Qed.
 
-(** The main theorem stating that interp_state preserves sbisim. *)
+(** The main theorem stating that fold_state preserves sbisim. *)
 
-Theorem interp_state_sbisim_gen {E F X Y} (h : E ~> stateT S (ctree F)) (Hh : forall X e s, vsimple (h X e s)) :
+Theorem fold_state_sbisim_gen {E F X Y} (h : E ~> stateT S (ctree F)) (Hh : forall X e s, vsimple (h X e s)) :
   forall s (k k' : X -> ctree E Y) (pre pre' : ctree F X),
   (forall x, sbisim (k x) (k' x)) ->
   pre ≅ pre' ->
   vsimple pre ->
-  sbisim (a <- pre;; Guard (interp_state h (k a) s)) (a <- pre';; Guard (interp_state h (k' a) s)).
+  sbisim (a <- pre;; Guard (fold_state h (k a) s)) (a <- pre';; Guard (fold_state h (k' a) s)).
 Proof.
   revert X. coinduction R CH.
   symmetric using idtac.
   { intros. apply H; eauto.  intros. rewrite H0. reflexivity. now rewrite H1. red; now setoid_rewrite <- H1. }
-  assert (CH' : forall (t t' : ctree E Y) s, t ~ t' -> st R (interp_state h t s) (interp_state h t' s)).
+  assert (CH' : forall (t t' : ctree E Y) s, t ~ t' -> st R (fold_state h t s) (fold_state h t' s)).
   {
     intros.
-    assert (st R (a <- Ret tt;; Guard (interp_state h ((fun _ => t) a) s))
-      (a <- Ret tt;; Guard (interp_state h ((fun _ => t') a) s))).
+    assert (st R (a <- Ret tt;; Guard (fold_state h ((fun _ => t) a) s))
+      (a <- Ret tt;; Guard (fold_state h ((fun _ => t') a) s))).
     { apply CH; eauto. left; eauto. }
     setoid_rewrite bind_ret_l in H0.
     rewrite !sb_guard in H0.
@@ -540,7 +539,7 @@ Proof.
   }
   intros. setoid_rewrite <- H0. clear pre' H0. cbn. intros.
   copy H0. rewrite bind_tau_r in H0.
-  eapply trans_interp_state_inv_gen in H0 as (? & ? & ? & ?); auto.
+  eapply trans_fold_state_inv_gen in H0 as (? & ? & ? & ?); auto.
   2: { destruct H1 as [[] | []]; rewrite H1.
     rewrite bind_ret_l. apply is_simple_guard_ret.
     rewrite bind_trigger. right. intros. inv_trans. subst.
@@ -557,7 +556,7 @@ Proof.
       rewrite <- H5 in H4. inv H4. 2: { step in H6. inv H6. }
       step in H3. inv H3. clear x2 H2 t H5.
       rewrite bind_trigger in cpy. apply trans_vis_inv in cpy. destruct cpy as (? & ? & ?). subst.
-      exists (Guard (interp_state h (k' x1) s)). rewrite H1. rewrite bind_trigger. now constructor.
+      exists (Guard (fold_state h (k' x1) s)). rewrite H1. rewrite bind_trigger. now constructor.
       rewrite H2, !sb_guard. apply CH'. apply H.
   - destruct H2 as (? & ? & ? & ?).
     destruct H1 as [[] | []]. 2: { rewrite H1 in H2. setoid_rewrite bind_trigger in H2. inv_trans. }
@@ -565,20 +564,20 @@ Proof.
     eapply transis_sbisim in H4; eauto. destruct H4 as (? & ? & ?).
     apply transis_trans in H2 as (? & ? & ?); auto.
     exists x3. rewrite H1, bind_ret_l. etrans.
-    assert (st R (interp_state h x x0) (interp_state h x1 x0)).
+    assert (st R (fold_state h x x0) (fold_state h x1 x0)).
     { apply CH'. apply H4. }
     rewrite sbisim_t0_det. 2: apply H0.
     setoid_rewrite sbisim_t0_det at 3. 2: apply H5.
     apply H6.
 Qed.
 
-#[global] Instance interp_state_sbisim {E F R} (h : E ~> stateT S (ctree F)) (Hh : forall X e s, vsimple (h X e s)) :
-  Proper (sbisim ==> eq ==> sbisim) (interp_state h (T := R)).
+#[global] Instance fold_state_sbisim {E F R} (h : E ~> stateT S (ctree F)) (Hh : forall X e s, vsimple (h X e s)) :
+  Proper (sbisim ==> eq ==> sbisim) (fold_state h (T := R)).
 Proof.
   cbn. intros. subst.
-  assert (a <- Ret tt;; Guard (interp_state h ((fun _ => x) a) y0) ~
-    a <- Ret tt;; Guard (interp_state h ((fun _ => y) a) y0)).
-  apply interp_state_sbisim_gen; auto.
+  assert (a <- Ret tt;; Guard (fold_state h ((fun _ => x) a) y0) ~
+    a <- Ret tt;; Guard (fold_state h ((fun _ => y) a) y0)).
+  apply fold_state_sbisim_gen; auto.
   red; eauto.
   setoid_rewrite bind_ret_l in H0. rewrite !sb_guard in H0. apply H0.
 Qed.
@@ -589,5 +588,5 @@ End State.
 Arguments get {S E _}.
 Arguments put {S E _}.
 Arguments run_state {S E} [_] _ _.
-Arguments interp_state {E C M S FM MM IM} h h' [T].
+Arguments fold_state {E C M S FM MM IM} h h' [T].
 
